semantics of checkers now depend on size as well

src/EndToEnd.v
@@ -18,20 +18,28 @@ Definition success qp :=
 
 (* Maps a Checker to a Prop *)
 Definition semChecker (P : Checker) : Prop :=
-  forall qp, semGen P qp -> success qp = true.
+  forall s qp, semSize P s qp -> success qp = true.
+
+Definition semCheckerSize (P : Checker) (s : nat): Prop :=
+  forall qp, semSize P s qp -> success qp = true.
 
 (* Maps a Checkable to a Prop i.e. gives an equivalent proposition to the
    property under test *)
 Definition semCheckable {A : Type} {_ : Checkable  A} (a : A) : Prop :=
   semChecker (checker a).
 
+Definition semCheckableSize {A : Type} {_ : Checkable  A} 
+           (a : A) (s : nat) : Prop :=
+  semCheckerSize (checker a) s.
+
 Lemma mapTotalResult_id:
-  forall {prop : Type} {H : Checkable prop} (f : Result -> Result) (p : prop),
+  forall {prop : Type} {H : Checkable prop} (f : Result -> Result) 
+         (p : prop) (s : nat),
     (forall res, resultSuccessful res = resultSuccessful (f res)) ->
-    (semChecker (mapTotalResult f p) <-> semCheckable p).
+    (semCheckerSize (mapTotalResult f p) s <-> semCheckableSize p s).
 Proof.
-  move => prop H f p Hyp.
-  rewrite /semCheckable  /mapTotalResult /mapRoseResult /mapProp /semChecker.
+  move => prop H f p s Hyp.
+  rewrite /semCheckable /mapTotalResult /mapRoseResult /mapProp /semChecker.
   split.
   - move=> H1 qp Hprop.
     set qp' :=
@@ -40,15 +48,15 @@ Proof.
       end.
     specialize (H1 qp'). 
     have: success qp' = true.
-    { apply H1.  apply semFmap. exists qp; split => //. }
+    { apply H1.  apply semFmapSize. exists qp; split => //. }
     destruct qp as [[]]. simpl in *. by rewrite -Hyp.
-  - move => H1 qp /semFmap [qp' [/H1 Hprop H2]]; subst.
+  - move => H1 qp /semFmapSize [qp' [/H1 Hprop H2]]; subst.
     destruct qp' as [[]]. simpl in *. by rewrite -Hyp.
 Qed.
 
 Lemma semCallback_id:
-  forall {prop : Type} {H : Checkable prop} (cb : Callback) (p : prop),
-    semChecker (callback cb p) <-> semCheckable p.
+  forall {prop : Type} {H : Checkable prop} (cb : Callback) (p : prop) (s : nat),
+    semCheckerSize (callback cb p) s <-> semCheckableSize p s.
 Proof.
   move => prop tp cb p. rewrite /callback.
   split; move => H.
@@ -59,56 +67,62 @@ Proof.
 Qed.
 
 Lemma semWhenFail_id:
-  forall {prop : Type} {H : Checkable prop} (s : String.string) (p : prop),
-    semChecker (whenFail s p) <-> semCheckable p.
+  forall {prop : Type} {H : Checkable prop} (s : String.string) (p : prop) 
+         (size : nat),
+    semCheckerSize (whenFail s p) size <-> semCheckableSize p size.
 Proof.
-  move => prop H s p. by rewrite /whenFail semCallback_id.
+  move => prop H s p size. by rewrite /whenFail semCallback_id.
 Qed.
 
 
 Lemma semPrintTestCase_id:
-  forall {prop: Type} {tp : Checkable prop} (s: String.string) (p: prop),
-    semChecker (printTestCase s p) <-> semCheckable p.
+  forall {prop: Type} {tp : Checkable prop} (s: String.string) 
+         (p: prop) (size : nat),
+    semCheckerSize (printTestCase s p) size <-> semCheckableSize p size.
 Proof.
-  move => prop tp s p. by rewrite /printTestCase semCallback_id.
+  move => prop tp s p size. by rewrite /printTestCase semCallback_id.
 Qed.
 
 
+Axiom semSizeCorrect :
+  forall A (g : G A) (x : A) size,
+    semSize g size x <-> exists seed, run g seed size = x.
 
 
 (* TODO : This proof needs refactoring! *)
 Lemma semShrinking_id:
   forall {prop A : Type} {H : Checkable prop}
-         (shrinker : A -> list A) (x0 : A) (pf : A -> prop),
-    semChecker (shrinking shrinker x0 pf) <->
-    semCheckable (pf x0).
+         (shrinker : A -> list A) (x0 : A) (pf : A -> prop) (s : nat),
+    semCheckerSize (shrinking shrinker x0 pf) s <->
+    semCheckableSize (pf x0) s.
 Proof.
-  move => prop A HCheck sh x pf. unfold semCheckable, shrinking, semChecker.
+  move => prop A HCheck sh x pf. 
+  unfold semCheckableSize, shrinking, semCheckerSize.
   split. 
   - unfold props. generalize 1000.  
-    case => [| n] H qp /semGenCorrect [size [seed Hgen]]; subst. 
-    + apply H. apply semFmap. eexists.
-      split. apply semPromote.  
-      exists seed. exists size. simpl. reflexivity.
+    case => [| n] H qp /semSizeCorrect [seed Hgen]; subst. 
+    + apply H. apply semFmapSize. eexists.
+      split. apply semPromoteSize.  
+      exists seed. simpl. reflexivity.
       simpl.
-      by destruct ((run (checker (pf x)) seed size)) as [[res [l]]] => /=.
+      by destruct ((run (checker (pf x)) seed s)) as [[res [l]]] => /=.
     + suff :
         success
           (run
              (fmap
                 (fun x0 => {| unProp := joinRose (fmapRose unProp x0) |})
-                (promote (@props' _ _ HCheck (S n) pf sh x))) seed size) = true.
+                (promote (@props' _ _ HCheck (S n) pf sh x))) seed s) = true.
       remember 
         (run
            (fmap
               (fun x0 : Rose QProp =>
                  {| unProp := joinRose (fmapRose unProp x0) |})
-              (promote (props' (S n) pf sh x))) seed size) as b.  
+              (promote (props' (S n) pf sh x))) seed s) as b.  
       symmetry in Heqb. setoid_rewrite runFmap in Heqb.
       move : Heqb => [rqp [Hrun Hb]]. simpl. rewrite Hb. 
       apply runPromote in Hrun. rewrite -Hrun. 
-      simpl in *. by destruct ((run (checker (pf x)) seed size)) as [[res [l]]] => /=.
-      apply H; exists size. 
+      simpl in *. by destruct ((run (checker (pf x)) seed s)) as [[res [l]]] => /=.
+      apply H.
       apply semFmapSize. eexists. split => /=.
       apply semPromoteSize.  exists seed. reflexivity.
       simpl. rewrite runFmap. eexists. split => //=.
@@ -116,25 +130,25 @@ Proof.
                      (promote
                         (MkRose (checker (pf x))
                            {| force := List.map (props' n pf sh) (sh x) |}))
-                     seed size)) as b.
+                     seed s)) as b.
       symmetry in Heqb. setoid_rewrite runPromote in Heqb. by rewrite -Heqb.
   - unfold props. generalize 1000.  
-    move => n H qp /semGenCorrect [size [seed /runFmap [rqp [H1 H2]]]].
-    suff : success (run (@checker _ HCheck (pf x)) seed size) = true.
+    move => n H qp /semSizeCorrect [seed /runFmap [rqp [H1 H2]]].
+    suff : success (run (@checker _ HCheck (pf x)) seed s) = true.
     + subst.
-      remember (run (promote (props' n pf sh x)) seed size) as b. symmetry in Heqb.
+      remember (run (promote (props' n pf sh x)) seed s) as b. symmetry in Heqb.
       apply runPromote in Heqb; subst. simpl.
       case: n => [| n] /=;
-      by destruct ((run (checker (pf x)) seed size)) as [[res [l]]] => //=.
-      subst. apply H. apply semGenCorrect.
+      by destruct ((run (checker (pf x)) seed s)) as [[res [l]]] => //=.
+      subst. apply H. apply semSizeCorrect.
       by eexists; eexists.
 Qed.
 
 
 Lemma semCover_id:
   forall {prop : Type} {H : Checkable prop} (b: bool) (n: nat)
-         (s: String.string) (p : prop),
-    semChecker (cover b n s p) <-> semCheckable p.
+         (s: String.string) (p : prop) (size: nat),
+    semCheckerSize (cover b n s p) size <-> semCheckableSize p size.
 Proof.
   move=> prop H b n s p. split.
   - rewrite /cover. case: b => //.
@@ -147,187 +161,193 @@ Qed.
 
 Lemma semClassify_id:
    forall {prop : Type} {H : Checkable prop} (b: bool) (s: String.string)
-          (p : prop),
-    semChecker (classify b s p) <-> semCheckable p.
+          (p : prop) (size : nat),
+    semCheckerSize (classify b s p) size <-> semCheckableSize p size.
 Proof.
-  move=> prop H b s p. by rewrite /classify semCover_id.
+  move=> prop H b s p size. by rewrite /classify semCover_id.
 Qed.
 
 Lemma semLabel_id:
    forall {prop : Type} {H : Checkable prop} (s: String.string)
-          (p : prop),
-    semChecker (label s p) <-> semCheckable p.
+          (p : prop) (size: nat),
+    semCheckerSize (label s p) size <-> semCheckableSize p size.
 Proof.
-  move=> prop H s p. by rewrite /label semClassify_id.
+  move=> prop H s p size. by rewrite /label semClassify_id.
 Qed.
 
 Lemma semCollect_id:
    forall {prop : Type} {H : Checkable prop} (s: String.string)
-          (p : prop),
-    semChecker (collect s p) <-> semCheckable p.
+          (p : prop) (size: nat),
+    semCheckerSize (collect s p) size <-> semCheckableSize p size.
 Proof.
-  move=> prop H s p. by rewrite /collect semLabel_id.
+  move=> prop H s p size. by rewrite /collect semLabel_id.
 Qed.
 
 Open Scope Checker_scope.
 
 Lemma semImplication:
       forall {prop : Type} {H : Checkable prop}
-             (p : prop) (b : bool),
-        semChecker (b ==> p) <-> b = true -> semCheckable p.
+             (p : prop) (b : bool) (s : nat),
+        semCheckerSize (b ==> p) s <-> b = true -> semCheckableSize p s.
 Proof.
   move => prop H p b. case: b.
   - split => /=; auto. apply. reflexivity.
   - split; try congruence. move => _.
     rewrite /implication.  rewrite /semChecker /checker /testResult.
-    move => qp. by move=> /semReturn H'; subst. 
+    move => qp . by move=> /semReturnSize H'; subst. 
 Qed.
   
 
 (* equivalences for other combinators *)
 
 Lemma semReturnGen:
-  forall (p : QProp),
-    semChecker (returnGen p) <-> semCheckable p.
+  forall (p : QProp) (size: nat),
+    semCheckerSize (returnGen p) size <-> semCheckableSize p size.
 Proof.
-  move=> p. rewrite /semChecker. split;
-  move => H qp Hprop; auto.
+  move=> qp s. rewrite /semChecker. split;
+  move => H qp' /semReturnSize Hprop; subst;
+  apply H; by apply semReturnSize. 
 Qed.
 
-(* Not provable *)
-(* Lemma semBindGen: *)
-(*   forall {A } (gen : G A) (p : A -> Checker), *)
-(*     semChecker (bindGen gen p) <->  *)
-(*     forall g, semGen gen g -> semChecker (p g). *)
-(* Proof.  *)
-(*   move => A gen p. unfold semChecker; split.  *)
-(* Abort. *)
-
+Lemma semBindGen:
+  forall {A } (gen : G A) (p : A -> Checker) (size: nat),
+    semCheckerSize (bindGen gen p) size <->
+    forall g, semSize gen size g -> semCheckerSize (p g) size.
+Proof.
+  move => A gen p. unfold semCheckerSize. split.
+  - move => H g Hsize qp Hsize'. eapply H.
+    apply semBindSize.  eexists; split; eassumption.
+  - move => H qp /semBindSize [a [H1 H2]]. eapply H; eassumption.
+Qed.
 
 Lemma semPredQProp:
-  forall (p : G QProp), semCheckable p <-> (semChecker p).
+  forall (p : G QProp) (s : nat), 
+    semCheckableSize p s <-> (semCheckerSize p s).
 Proof.
-   move=> p.
-  rewrite /semCheckable /checker /testGenProp /checker /testProp /semChecker.
+  move=> p.
+  rewrite /semCheckableSize /checker 
+          /testGenProp /checker /testProp /semCheckerSize.
   split.
-  - move => Hqp qp [s Hsize]. apply Hqp. exists s.
+  - move => Hqp qp Hsize. apply Hqp. 
     apply semBindSize. exists qp. split => //.
     by apply semReturnSize.
-  - move => H pq [s /semBindSize [qp [H1 /semReturnSize H2]]]; subst.
-    apply H. by exists s.
+  - move => H pq /semBindSize [qp [H1 /semReturnSize H2]]; subst.
+    by apply H.
 Qed.
 
 Lemma semForAll :
   forall {A prop : Type} {H : Checkable prop} `{Show A} 
-         (gen : G A) (f : A -> prop),
-    semChecker (forAll gen f) <->
-    forall (a : A) s, semSize gen s a -> semCheckable (f a).
+         (gen : G A) (f : A -> prop) (size: nat),
+    semCheckerSize (forAll gen f) size <->
+    forall (a : A), semSize gen size a -> semCheckableSize (f a) size.
 Proof.
-  (* move => A prop Htest show gen pf. split => H'. *)
-  (* - rewrite /forAll  /semCheckable /semChecker in H'.  *)
-  (*   move : H' => H' a S Hgen. *)
-  (*   rewrite /semCheckable /semChecker => qp [s' Hgen']. *)
-  (*   apply H'. eexists. apply semBindSize. eexists; split => //. *)
-  (*   apply Hgen. apply semPrintTestCase_id. *)
-  (*   apply semPrintTestCase_id in Hgen. *)
-  (* - rewrite /forAll in H' *. apply semBindGen => g Hgen. *)
-  (*   rewrite semPrintTestCase_id. by apply H'. *)
-Abort.
+  move => A prop Htest show gen pf. split => H'.
+  - rewrite /forAll in H'. move/semBindGen : H' => H' a /H' Hgen.
+    by apply semPrintTestCase_id in Hgen.
+  - rewrite /forAll in H' *. apply semBindGen => g Hgen.
+    rewrite semPrintTestCase_id. by apply H'.
+Qed.
 
 Lemma semForAllShrink:
   forall {A prop : Type} {H : Checkable prop} `{Show A}
-         (gen : G A) (f : A -> prop) shrinker,
-    semChecker (forAllShrink gen shrinker f) <->
-    forall a : A, semGen gen a -> semCheckable (f a).
+         (gen : G A) (f : A -> prop) shrinker (size: nat),
+    semCheckerSize (forAllShrink gen shrinker f) size <->
+    forall a : A, semSize gen size a -> semCheckableSize (f a) size.
 Proof.
-  (* move => A prop H show gen pf shrink. split. *)
-  (* - rewrite /forAllShrink semBindGen. *)
-  (*   move=> H' a /H' Hgen. setoid_rewrite semShrinking_id in Hgen. *)
-  (*   setoid_rewrite semPredQProp in Hgen. *)
-  (*   by apply semPrintTestCase_id in Hgen. *)
-  (* - move=> H'. rewrite /forAllShrink semBindGen. move => a g. *)
-  (*   rewrite semShrinking_id. apply semPredQProp. *)
-  (*   rewrite semPrintTestCase_id. by auto. *)
-Abort.
+  move => A prop H show gen pf shrink. split.
+  - rewrite /forAllShrink semBindGen.
+    move=> H' a /H' Hgen. setoid_rewrite semShrinking_id in Hgen.
+    setoid_rewrite semPredQProp in Hgen.
+    by apply semPrintTestCase_id in Hgen.
+  - move=> H'. rewrite /forAllShrink semBindGen. move => a g.
+    rewrite semShrinking_id. apply semPredQProp.
+    rewrite semPrintTestCase_id. by auto.
+Qed.
+
 
 (* equivalent Props for Checkables *)
 
 Lemma semBool:
-  forall (b : bool), semCheckable b <-> b = true.
+  forall (b : bool) (size: nat), semCheckableSize b size <-> b = true.
 Proof.  
   move => b. case: b. 
-  - split => //. rewrite /semCheckable /semChecker.
-    by move => _ qp [size /semReturnSize Heq]; subst.
-  - split => //. rewrite /semCheckable /semChecker. 
+  - split => // _. rewrite /semCheckableSize /semCheckerSize. 
+    by move => qp /semReturnSize Heq; subst.
+  - split => //. rewrite /semCheckableSize /semCheckerSize. 
     move => /(_ (MkProp (MkRose (liftBool false) (lazy nil)))) H.
-    apply H. by apply semReturn. 
+    apply H. by apply semReturnSize.
 Qed.
 
 Lemma semResult:
-  forall (res: Result), semCheckable res <-> resultSuccessful res = true.
+  forall (res: Result) (size: nat), 
+    semCheckableSize res size <-> resultSuccessful res = true.
 Proof.
-  rewrite /semCheckable /checker /testResult /semChecker.
+  rewrite /semCheckableSize /checker /testResult /semCheckerSize.
   move => res. split.
   + move=> /(_ ({| unProp := returnRose res |})) /= H.
-    apply H. by apply semReturn.
-  + by move=> H [[res' l]] [Heq1 /semReturnSize [Heq2 Heq3]]; subst. 
+    apply H. by apply semReturnSize.
+  + by move=> H [[res' l]] /semReturnSize [Heq2 Heq3]; subst. 
 Qed.
 
 Lemma semUnit:
-  forall (t: unit), semCheckable t <-> True.
+  forall (t: unit) (size: nat), semCheckableSize t size <-> True.
 Proof.
   move => t. split => // _.
-  by move => qp /semReturn Heq; subst. 
+  by move => qp /semReturnSize Heq; subst. 
 Qed.
 
 Lemma semQProp:
-  forall (qp: QProp), semCheckable qp <-> success qp = true.
+  forall (qp: QProp) (size: nat), 
+    semCheckableSize qp size <-> success qp = true.
 Proof.
   move => qp. 
-  rewrite /semCheckable /semChecker /checker /testProp.
+  rewrite /semCheckableSize /semCheckerSize /checker /testProp.
   split. 
-  - apply. by apply semReturn.
-  - by move => H qp' /semReturn Heq; subst.
+  - apply. by apply semReturnSize.
+  - by move => H qp' /semReturnSize Heq; subst.
 Qed.
 
 Lemma semGen:
-  forall (P : Type) {H : Checkable P} (gen: G P),
-    (semCheckable gen) <-> (forall p, semGen gen p -> semCheckable p).
+  forall (P : Type) {H : Checkable P} (gen: G P) (size : nat),
+    (semCheckableSize gen size) <-> 
+    (forall p, semSize gen size p -> semCheckableSize p size).
 Proof.
-  move=> P H gen. split.
-  - move=> Hsem qp [n1 Hgen]. rewrite /semCheckable /semChecker in Hsem *.
-    move => qp' [n2 Hprop]. simpl in *.
-    apply Hsem. exists n1. apply semBindSize. exists qp.
-    split => //.
-Abort.
+  move=> P H gen. unfold semCheckableSize, semCheckerSize in *. split.
+  - move=> Hsem qp Hsize. 
+    move => qp' Hprop. simpl in *.
+    apply Hsem. apply semBindSize. exists qp.
+    by split => //.
+  - move => Hsem qp /semBindSize [p [Hsize Hsize']]. 
+    eapply Hsem; eassumption. 
+Qed.
 
 Lemma semFun:
   forall {A prop : Type} {H1 : Show A} {H2 : Arbitrary A} {H3 : Checkable prop}
-         (f : A -> prop),
-    semCheckable f <->
-    forall (a : A), semGen arbitrary a -> semCheckable (f a).
+         (f : A -> prop) (size: nat),
+    semCheckableSize f size <->
+    forall (a : A), semSize arbitrary size a -> semCheckableSize (f a) size.
 Proof.
-  (* move=> A prop H1 H2 H3 f. *)
-  (* rewrite /semCheckable /checker /testFun. *)
-  (* split. *)
-  (* - move => /semForAllShrink H' a' /H' Gen. by auto. *)
-  (* - move => H'. apply semForAllShrink => a' /H' Hgen. by auto. *)
-Abort.
+  move=> A prop H1 H2 H3 f.
+  rewrite /semCheckable /checker /testFun.
+  split.
+  - move => /semForAllShrink H' a' /H' Gen. by auto.
+  - move => H'. apply semForAllShrink => a' /H' Hgen. by auto.
+Qed.
 
-(* I think this is the strongest checker we can get for polymorphic functions *)
 Lemma semPolyFun:
-  forall {prop : Type -> Type} {H : Checkable (prop nat)} (f : forall T, prop T),
-    (semCheckable f) <-> (semCheckable (f nat)).
+  forall {prop : Type -> Type} {H : Checkable (prop nat)} (f : forall T, prop T)
+         (size : nat),
+    (semCheckableSize f size) <-> (semCheckableSize (f nat) size).
 Proof.
-  move => prop H f. rewrite /semCheckable {2}/checker /testPolyFun.
+  move => prop H f s. rewrite /semCheckableSize {2}/checker /testPolyFun.
   by rewrite semPrintTestCase_id.
 Qed.
 
 Lemma semPolyFunSet:
-  forall {prop : Set -> Type} {H : Checkable (prop nat)} (f : forall T, prop T),
-    (semCheckable f) <->  (semCheckable (f nat)).
+  forall {prop : Set -> Type} {H : Checkable (prop nat)} (f : forall T, prop T) (size: nat),
+    (semCheckableSize f size) <->  (semCheckableSize (f nat) size).
 Proof.
-  move => prop H f. rewrite /semCheckable {2}/checker /testPolyFun.
+  move => prop H f s. rewrite /semCheckableSize {2}/checker /testPolyFun.
   by rewrite semPrintTestCase_id.
 Qed.
 
@@ -336,13 +356,13 @@ Qed.
 
 Class Provable (A : Type) {H: Checkable A} : Type :=
  {
-    proposition : A -> Prop;
-    _ : forall a, proposition a <-> semCheckable a
+    proposition : nat -> A -> Prop;
+    _ : forall a s, proposition s a <-> semCheckableSize a s
   }.
 
 Program Instance proveResult : Provable Result :=
   {|
-    proposition := resultSuccessful
+    proposition s r := resultSuccessful r
   |}.
 Next Obligation.
   by rewrite semResult.
@@ -350,7 +370,7 @@ Qed.
 
 Program Instance proveUnit : Provable unit :=
   {|
-    proposition := fun _ => True
+    proposition := fun _ _ => True
   |}.
 Next Obligation.
   by rewrite semUnit.
@@ -358,7 +378,7 @@ Qed.
 
 Program Instance proveQProp : Provable QProp :=
   {|
-    proposition qp := success qp = true
+    proposition s qp := success qp = true
   |}.
 Next Obligation.
   by rewrite semQProp.
@@ -366,42 +386,43 @@ Qed.
 
 Program Instance proveBool : Provable bool :=
   {|
-    proposition b :=  b = true
+    proposition s b :=  b = true
   |}.
 Next Obligation.
   by rewrite semBool.
 Qed.
 
-(* Program Instance proveGenProp {prop : Type} `{Provable prop} : *)
-(*   Provable (G prop) := *)
-(*   {| *)
-(*     proposition g := (forall p, semGen g p -> proposition p) *)
-(*   |}. *)
-(* Next Obligation. *)
-  (* destruct H0 as [semP proof]. rewrite /proposition. split. *)
-  (* - move => H'. apply semGen=> p Hgen. apply proof. by auto. *)
-  (* - move => /semGen H' p Hgen. apply proof. by auto. *)
-(* Abort. *)
+Program Instance proveGenProp {prop : Type} `{Provable prop} :
+  Provable (G prop) :=
+  {|
+    proposition s g := (forall p, semSize g s p -> proposition s p)
+  |}.
+Next Obligation.
+  destruct H0 as [semP proof]. rewrite /proposition. split.
+  - move => H'. apply semGen=> p Hgen. apply proof. eapply H'. eassumption. 
+  - move => /semGen H' p Hgen. eapply proof. apply H'. by auto.
+Qed.
 
-(* Program Instance proveFun {A prop: Type} `{Arbitrary A} `{Show A} *)
-(*         `{Provable prop}: Provable (A -> prop) := *)
-(*   {| *)
-(*     proposition p := *)
-(*       (forall a, *)
-(*          semGen arbitrary a -> *)
-(*          proposition (p a)) *)
-(*   |}. *)
-(* Next Obligation. *)
-(*   destruct H2 as [semP proof]. rewrite /proposition. split. *)
-(*   - move=> H'. apply semFun => a' /H' Hgen. *)
-(*     by apply proof. *)
-(*   - move=> H' a' Hgen. apply proof. by apply semFun. *)
-(* Qed. *)
+
+Program Instance proveFun {A prop: Type} `{Arbitrary A} `{Show A}
+        `{Provable prop}: Provable (A -> prop) :=
+  {|
+    proposition s p :=
+      (forall a,
+         semSize arbitrary s a ->
+         proposition s (p a))
+  |}.
+Next Obligation.
+  destruct H2 as [semP proof]. rewrite /proposition. split.
+  - move=> H'. apply semFun => a' /H' Hgen.
+    by apply proof.
+  - move=> H' a' Hgen. apply proof. by apply semFun.
+Qed.
 
 Program Instance provePolyFun {prop : Type -> Type} `{Provable (prop nat)} :
   Provable (forall T, prop T) :=
   {
-    proposition f := proposition (f nat)
+    proposition s f := proposition s (f nat)
   }.
 Next Obligation.
   destruct H0 as [semP proof]. rewrite /proposition. split.
@@ -412,7 +433,7 @@ Qed.
 Program Instance provePolyFunSet {prop : Set -> Type} `{Provable (prop nat)} :
   Provable (forall T, prop T) :=
   {
-    proposition f := proposition (f nat)
+    proposition s f := proposition s (f nat)
   }.
 Next Obligation.
   destruct H0 as [semP proof]. rewrite /proposition. split.
